theories/type_checker_reflects_typing.v
@@ -17,6 +17,56 @@ Proof.
   rewrite subn0. apply/eqP. by apply drop_size.
 Qed.
 
+Print upd_local_label_return.
+
+Lemma upd_label_overwrite: forall C loc lab ret lab',
+  upd_label (upd_local_label_return C loc lab ret) lab'
+  = upd_local_label_return C loc lab' ret.
+Proof.
+  move => C loc lab ret lab'.
+  unfold upd_label.
+  unfold upd_local_label_return. by auto.
+Qed.
+
+(*???*)
+Ltac bool_to_prop_and:=
+  repeat match goal with
+         | H: _ && _ = true |- _ =>
+           move/andP in H; destruct H
+         | H: _ && _ |- _ =>
+           move/andP in H; destruct H
+end.
+
+(*
+  Let's first state this lemma which naturally sounds correct.
+*)
+
+Lemma inst_typeP:
+  forall s i C,
+    reflect (inst_type_check s i = C) (inst_typing s i C).
+Proof.
+  move => s i C. destruct (inst_typing s i C) eqn:itc_bool => //=.
+  - apply ReflectT. unfold inst_typing in itc_bool.
+    destruct i. destruct C. destruct tc_local => //=. destruct tc_label => //=.
+    destruct tc_return => //=.
+    unfold inst_type_check => /=.
+    bool_to_prop_and.
+    (**TODO**)
+    move/andP in H. destruct H as [H H1].
+    move/andP in H. destruct H as [H H2].
+    move/andP in H. destruct H as [H H3].
+    move/eqP in H. rewrite H. clear H.
+    (**---**)
+    admit.
+  - admit.
+Admitted.
+
+(* 
+  This seems really non-trivial. The structrue might also change after we fix
+    the duplication in the definition of be_type_check. How about we leave this
+    as admitted for now and explore other things first?
+*)
+
 Lemma wasm_type_checker_reflects_typing:
   forall C es,
     reflect (cl_typing_self C es) (cl_type_check C es).
@@ -30,10 +80,11 @@ Proof.
     + move => _. by apply cl_typing_host.
   - apply ReflectF. move => tc_prop.
     assert (cl_type_check C es = true) as HTest; last by rewrite tc_bool in HTest.
-    clear tc_bool.
-    unfold cl_typing_self in tc_prop.
+    clear tc_bool. move:tc_prop. move:es.
+    
+    unfold cl_typing_self.
+    move => es tc_prop.
     inversion tc_prop; subst => //=.
-    unfold c_types_agree.
     clear H5.
     (* This is important as otherwise Coq will fail to remember this information
          and the proof cannot be done otherwise. It's in SF but this is also a 
@@ -41,12 +92,13 @@ Proof.
 https://stackoverflow.com/questions/4519692/keeping-information-when-using-induction
     *)
     remember (Tf [::] t2s) as tf.
-    clear tc_prop.
+    unfold cl_type in tc_prop.
     induction H2; subst => //.
     + inversion Heqtf. by apply/eqP.
-    + simpl. by rewrite ct_suffix_empty.
-    + inversion Heqtf. by apply/eqP.
-    + simpl.
+    + simpl. unfold type_update => /=. rewrite ct_suffix_empty => /=.
+      by rewrite ct_suffix_empty.
+    + inversion Heqtf; subst. admit.
+    + simpl. admit.
 
     
 Admitted. (* TODO *)
