theories/type_soundness.v
@@ -1,0 +1,90 @@
+Require Import common.
+From mathcomp Require Import ssreflect ssrfun ssrnat ssrbool eqtype seq.
+
+Set Implicit Arguments.
+Unset Strict Implicit.
+Unset Printing Implicit Defensive.
+
+Require Import operations typing datatypes_properties typing opsem.
+
+Definition b_to_a (bes: seq basic_instruction) : seq administrative_instruction :=
+  map (fun x => (Basic x)) bes.
+
+Definition a_to_b_single (e: administrative_instruction) : basic_instruction :=
+  match e with
+  | Basic x => x
+  | _ => EConst (ConstInt32 (Wasm_int.Int32.zero))
+  end.
+
+Definition a_to_b (es: seq administrative_instruction) : seq basic_instruction :=
+  map a_to_b_single es.
+
+Lemma b_a_elim: forall bes es,
+    es = b_to_a bes ->
+    bes = a_to_b es.
+Proof.
+  induction bes; move => es H => //=.
+  - by rewrite H.
+  - simpl in H. assert (es = b_to_a (a :: bes)) as H1.
+    + by rewrite H.
+    + rewrite H1. simpl. f_equal. by apply IHbes.
+Qed.   
+
+Definition t_be_value (es: seq basic_instruction) : Prop :=
+  const_list (b_to_a es).
+
+Print tc_global.
+
+(*
+  It is less trivial than thought to state this theorem because typing and opsem used
+    different parameters in their corresponding formulation.
+ *)
+
+Print value.
+
+Print value_type.
+
+Definition v_to_vt (v: value) :=
+  match v with
+  | ConstInt32 _ => T_i32
+  | ConstInt64 _ => T_i64
+  | ConstFloat32 _ => T_f32
+  | ConstFloat64 _ => T_f64
+  end.
+
+Definition vs_to_vts (vs: list value) :=
+  map v_to_vt vs.
+
+(* Questionable formulation on b_e only. cl_typing seems to already include 
+     be_typing and inst_typing?*)
+
+Theorem t_be_progress: forall C i s vs bes tf,
+    be_typing C bes tf ->
+    inst_typing s i C ->
+    vs_to_vts vs = tc_local C ->
+    (t_be_value bes \/
+     exists s' vs' es', reduce s vs (b_to_a bes) i s' vs' es').
+Proof.
+Admitted.
+
+Ltac b_to_a_revert :=
+  repeat lazymatch goal with
+         | H: _ = b_to_a ?bes |- _ =>
+           apply b_a_elim in H
+         end.
+
+(* This has a 0% chance of being the correct statement. I just wanted to see
+     how the opsem condition works when we do inversion on it. *)
+Theorem t_be_preservation: forall s vs bes i s' vs' bes' C C' tf,
+    reduce s vs (b_to_a bes) i s' vs' (b_to_a bes') ->
+    be_typing C bes tf ->
+    inst_typing s i C ->
+    vs_to_vts vs = tc_local C ->
+    inst_typing s' i C' ->
+    vs_to_vts vs' = tc_local C' ->
+    be_typing C' bes' tf.
+Proof.
+  move => s vs bes i s' vs' bes' C C' tf HOpsem HBET HInstT HLocalT HInstT' HLocalT'.
+  inversion HOpsem; subst.
+  - (* reduce_simple *)
+Admitted.
